We remind ourselves that we want to study the SIR model
\begin{equation*}
  \begin{split}
    \dv{S}{t}&=-rSI,\\
    \dv{I}{t}&=rSI-aI.\\
    \dv{R}{t}&=aI.\\    
    \end{split}
  \end{equation*}
  and we are looking for a generator of the following kind:
\begin{equation}
X=\xi(t,S,I,R)\partial_t+\eta_1(t,S,I,R)\partial_S+\eta_2(t,S,I,R)\partial_I+\eta_3(t,S,I,R)\partial_R.
\end{equation}
Now, the first linearised symmetry condition is
\begin{align}
  - a r I^{2} S \pdv{\xi}{I} + a r I^{2} S \pdv{\xi}{R} - a I \pdv{\eta_1}{I} + a I \pdv{\eta_1}{R}&\nonumber\\
  + r^{2} I^{2} S^{2} \pdv{\xi}{I} - r^{2} I^{2} S^{2} \pdv{\xi}{S} + r I S \pdv{\eta_1}{I} - r I S \pdv{\eta_1}{S} &\nonumber\\
  + r I S \pdv{\xi}{t} + r I \eta_1 + r S \eta_2 + \pdv{\eta_1}{t}=0\label{eq:SIR_lin_sym_1}
\end{align}
and the corresponding determining equations:
\begin{align}
1:&\pdv{\eta_1}{t}=0,\\
I:&- a \pdv{\eta_1}{I} + a \pdv{\eta_1}{R} + r \eta_1=0,\\
S:&r \eta_2=0,\\
S I:&r \pdv{\eta_1}{I} - r \pdv{\eta_1}{S} + r \pdv{\xi}{t}=0,\\
S I^{2}:&- a r \pdv{\xi}{I} + a r \pdv{\xi}{R}=0,\\
S^{2} I^{2}:&r^{2} \pdv{\xi}{I} - r^{2} \pdv{\xi}{S}=0.\\
\end{align}
Now, the second linearised symmetry condition is
\begin{align}
  - a^{2} I^{2} \pdv{\xi}{I} + a^{2} I^{2} \pdv{\xi}{R} + 2 a r I^{2} S \pdv{\xi}{I} - a r I^{2} S \pdv{\xi}{R}&\nonumber\\
  - a r I^{2} S \pdv{\xi}{S} - a I \pdv{\eta_2}{I} + a I \pdv{\eta_2}{R} + a I \pdv{\xi}{t}&\nonumber\\
  - r^{2} I^{2} S^{2} \pdv{\xi}{I} + r^{2} I^{2} S^{2} \pdv{\xi}{S} + r I S \pdv{\eta_2}{I} - r I S \pdv{\eta_2}{S}&\nonumber\\
  - r I S \pdv{\xi}{t} + r I \eta_1 + r S \eta_2 + \pdv{\eta_2}{t}=0\label{eq:SIR_lin_sym_2}
\end{align}
and the corresponding determining equations:

\begin{align}
1:&\pdv{\eta_2}{t}=0,\\
I:&- a \pdv{\eta_2}{I} + a \pdv{\eta_2}{R} + a \pdv{\xi}{t} + r \eta_1=0,\\
I^{2}:&- a^{2} \pdv{\xi}{I} + a^{2} \pdv{\xi}{R}=0\\
S:&r \eta_2=0,\\
S I:&r \pdv{\eta_2}{I} - r \pdv{\eta_2}{S} - r \pdv{\xi}{t}=0,\\
S I^{2}:&2 a r \pdv{\xi}{I} - a r \pdv{\xi}{R} - a r \pdv{\xi}{S}=0,\\
S^{2} I^{2}:&- r^{2} \pdv{\xi}{I} + r^{2} \pdv{\xi}{S}=0.\\
\end{align}
Now, the third linearised symmetry condition is
\begin{align}
  a^{2} I^{2} \pdv{\xi}{I} - a^{2} I^{2} \pdv{\xi}{R} - a r I^{2} S \pdv{\xi}{I} + a r I^{2} S \pdv{\xi}{S}&\nonumber\\
  - a I \pdv{\eta_3}{I} + a I \pdv{\eta_3}{R} - a I \pdv{\xi}{t} + r I S \pdv{\eta_3}{I}&\nonumber\\
  - r I S \pdv{\eta_3}{S} + r I \eta_1 + r S \eta_2 + \pdv{\eta_3}{t}=0\label{eq:SIR_lin_sym_3}
\end{align}
and the corresponding determining equations:
\begin{align}
1:&\pdv{\eta_3}{t}=0,\\
I:&- a \pdv{\eta_3}{I} + a \pdv{\eta_3}{R} - a \pdv{\xi}{t} + r \eta_1=0,\\
I^{2}:&a^{2} \pdv{\xi}{I} - a^{2} \pdv{\xi}{R}=0,\\
S:&r \eta_2=0,\\
S I:&r \pdv{\eta_3}{I} - r \pdv{\eta_3}{S}=0,\\
S I^{2}:&- a r \pdv{\xi}{I} + a r \pdv{\xi}{S}=0.
\end{align}